concurrency/hashtable/Interface.i.dfy
@@ -7,16 +7,40 @@ module FilledInInterface refines Interface(
   HashTableRefinement)
 {
   import opened Impl
+  import opened GhostLinearSequence_i
+  import opened CircularRange
+  import opened Limits
+
+  import opened Mutexes
 
   type SharedVars = IVariables
 
   predicate SharedWF(s: SharedVars)
+  {
+    s.Inv(TicketStubSingletonLoc.loc())
+  }
 
   method init(glinear in_token: T.Token)
   returns (linear s: SharedVars)
   //requires in_token.loc == TicketStubSingletonLoc.loc()
   //requires in_token.val == ssm.Init()
   ensures SharedWF(s)
+  {
+    linear var v: Variables;
+    v, s := Impl.init(in_token);
+    
+    forall i: Index 
+      ensures i !in v.handles
+    {
+      assert !v.HasRowHandle(i);
+    }
+
+    linear var Variables(
+      token, handles) := v;
+
+    glseq_delete(handles);
+    T.dispose(token);
+  }
 
   method do_operation(shared s: SharedVars,
       ghost rid: nat, input: MapIfc.Input, glinear ticket: T.Token)
@@ -25,4 +49,24 @@ module FilledInInterface refines Interface(
   //requires ticket.val == ssm.Ticket(rid, input)
   ensures stub.loc == TicketStubSingletonLoc.loc()
   ensures ssm.IsStub(rid, output, stub.val)
+  decreases *
+  {
+    glinear var fresh_handles := glseq_alloc<MutexHandle<Row>>(FixedSize());
+    linear var v := Variables(ticket, fresh_handles);
+
+    output := inout v.call(s, rid, input);
+
+    forall i: Index 
+      ensures i !in v.handles
+    {
+      assert !v.HasRowHandle(i);
+    }
+
+    linear var Variables(
+      token, handles) := v;
+
+    stub := token;
+    
+    glseq_delete(handles);
+  }
 }
